Working relations library

dafny/set-theory/binRelOnS.dfy
@@ -1,5 +1,8 @@
+include "binRelOnST.dfy"
+
 module binRelS
 {    
+    import opened binRelST
     /*
     Abstraction of a finite binary relation on a 
     set, S. Underlying representation is a pair: 
@@ -7,54 +10,75 @@ module binRelS
     */ 
     class binRelOnS<T(!new,==)>
     {
-        var d: set<T>;
-        var p: set<(T,T)>;
+        /*
+        We represent a binary relation, R, over a set,
+        T, as a value of the type of binary relations
+        over two types, but where both types are just S.
+        */
+        var r: binRelOnST<T,T>;
+
+        /*
+        This object is valid if it's a valid relation on
+        S X T and the domain and codomain are the same set.
+        */
         predicate Valid()
             reads this;
+            reads r;
         {
-            forall x, y :: (x, y) in p ==> x in d && y in d
+            r.Valid() && r.dom() == r.codom()
         }
 
+
         /*
-        Constructor requires that all values appearing in 
-        any of the pairs in p be in d. That is, the pairs
-        in p must represent a relation on domain, d. Note
-        that the "ensures d == dom && p == pairs" really is
-        needed here: the bodies of methods are not visible
-        globally within the class, so a visible postcondition
-        describing what the constructor does is needed to
-        enable verification that tasks need this knowledge.
+        Constructor just instantiates a binary relation
+        on S X T with the type, T, of the single set over
+        which the current relation is defined, setting the
+        domain and codomain sets to be the same set, elts.
         */
-        constructor(dom: set<T>, pairs: set<(T,T)>)
+        constructor(elts: set<T>, pairs: set<(T,T)>)
             requires forall x, y :: 
-                (x, y) in pairs ==> x in dom && y in dom;
-            ensures d == dom && p == pairs;
+                (x, y) in pairs ==> x in elts && y in elts;
+            ensures r.d == elts && 
+                    r.c == elts && r.r == pairs
             ensures Valid();
-        {
-            d := dom;
-            p := pairs;
+         {
+            r := new binRelOnST(elts,elts,pairs);
         }
 
         /*
-        Return domain/range set
+        Return domain set
         */
         function method dom(): set<T>
             reads this;
+            reads r;
             requires Valid();
             ensures Valid();
         {
-            d
+            r.dom()
+        }
+
+        /*
+        Return codomain set
+        */
+        function method codom(): set<T>
+            reads this;
+            reads r;
+            requires Valid();
+            ensures Valid();
+        {
+            r.codom()
         }
 
         /*
         Return set of ordered pairs
         */
         function method rel(): set<(T,T)>
-            reads this
+            reads this;
+            reads r;
             requires Valid();
             ensures Valid();
         {
-            p
+            r.rel()
         }
 
 
@@ -63,13 +87,11 @@ module binRelS
         */
         predicate method isFunction()
             reads this;
+            reads r;
             requires Valid();
             ensures Valid();
         {
-        forall x, y, z :: x in dom() && y in dom() && z in dom() &&
-                            (x, y) in rel() && 
-                            (x, z) in rel() ==> 
-                            y == z  
+            r.isFunction()  
         }
 
         
@@ -78,14 +100,12 @@ module binRelS
         */
         predicate method isInjective()
             reads this;
+            reads r;
             requires Valid();
             requires isFunction();
             ensures Valid();
         {
-        forall x, y, z :: x in dom() && y in dom() && z in dom() &&
-                            (x, z) in rel() && 
-                            (y, z) in rel() ==> 
-                            x == y  
+            r.isInjective()
         }
         
         
@@ -94,13 +114,13 @@ module binRelS
         */
         predicate method isSurjective()
             reads this;
+            reads r;
             requires Valid();
             requires isFunction();
             ensures Valid();
         {
-            (set x, y | x in dom() && y in dom() && (x, y) in rel() :: y) == dom()    
+            r.isSurjective()
         }
-
 
         /*
         Return true iff the relation a function and is bijective
@@ -108,11 +128,12 @@ module binRelS
 
         predicate method isBijective()
             reads this;
+            reads r;
             requires Valid();
             requires isFunction();
             ensures Valid();
         {
-            this.isInjective() && this.isSurjective()    
+            r.isBijective()    
         }
 
 
@@ -121,13 +142,11 @@ module binRelS
         */
         predicate method isTotal()
             reads this;
+            reads r;
             requires Valid();
-            ensures isTotal() ==> 
-                    (forall x :: x in dom() ==> 
-                        (exists y :: y in dom() && (x,y) in rel()))
             ensures Valid();
         {
-            (set x, y | x in dom() && y in dom() && (x, y) in rel() :: x) == dom()
+            r.isTotal()
         }
 
         
@@ -136,10 +155,11 @@ module binRelS
         */
         predicate method isPartial()
             reads this;
+            reads r;
             requires Valid();
             ensures Valid();
         {
-            !isTotal()
+            !r.isTotal()
         }
 
 
@@ -148,6 +168,7 @@ module binRelS
         */
         predicate method isReflexive()
             reads this;
+            reads r;
             requires Valid();
             ensures Valid();        
         {
@@ -160,6 +181,7 @@ module binRelS
         */
         predicate method isSymmetric()
             reads this;
+            reads r;
             requires Valid();
             ensures Valid();
         {
@@ -173,13 +195,15 @@ module binRelS
         */
         predicate method isTransitive()
             reads this;
+            reads r;
             requires Valid();
             ensures Valid();
         {
-            forall x, y, z ::  x in dom() && y in dom() && z in dom() &&
-                            (x, y) in rel() && 
-                            (y, z) in rel() ==> 
-                            (x, z) in rel() 
+            forall x, y, z ::  
+                x in dom() && y in dom() && z in dom() &&
+                (x, y) in rel() && 
+                (y, z) in rel() ==> 
+                (x, z) in rel() 
         }
 
 
@@ -187,5 +211,44 @@ module binRelS
         Exercise: formalize and implement a test for being
         an equivalence relation.
         */
+       predicate method isEquivalence()
+            reads this;
+            reads r;
+            requires Valid();
+            ensures Valid();
+        {
+            isReflexive() && isSymmetric() && isTransitive() 
+        }
+
+
+        /*
+        Compute image of a domain element under this relation.
+        */
+        function method image(k: T): (r: set<T>)
+            reads this;
+            reads r;
+            requires Valid(); 
+            ensures Valid();
+        {
+            r.image(k)
+        }
+
+
+
+        /*
+        Compute image of a domain element under this relation.
+        */
+        method imagef(k: T) returns (ret: T)
+            requires Valid(); 
+            requires isFunction();
+            requires isTotal();   // ensures defined for every value
+            requires k in dom();  // ensures function is non-empty
+            ensures ret in image(k);
+            ensures this == old(this);
+            ensures r == old(r);
+            ensures Valid();
+        {
+            ret := r.imagef(k);
+        }
     }
 }
