dafny/set-theory/binRelOnST.dfy
@@ -1,0 +1,273 @@
+module binRelST
+{    
+    /*
+    Abstraction of a finite binary relation on a 
+    set, S. Underlying representation is a triple: 
+    the domain set, S, the co-domain set, T, and 
+    a set of pairs over S X T.
+    */ 
+    class binRelOnST<S(!new,==),T(!new,==)>
+    {
+        var d: set<S>;      // domain: set of values of type S
+        var c: set<T>       // codomain: set of values of type T
+        var r: set<(S,T)>;  // relation: set of pairs from s X t
+        predicate Valid()
+            reads this;
+        {
+            // all tuple elements must be in dom and codom, respectively
+            forall x, y :: (x, y) in r ==> x in d && y in c
+        }
+
+        /*
+        Constructor requires that all values appearing in 
+        any of the pairs in p be in domain and codomain sets,
+        respectively. A note: the ensures clause really is
+        needed here: the bodies of *methods* are not visible
+        to the verifier, so if you want the verifier to be
+        able to use knowledge of what a method does, you must
+        make that behavior explicit in the specification. By
+        contrast, in Dafny, function bodies are visible to 
+        the verifier, though they can be made "opaque" using
+        a special keyword. 
+        */
+        constructor(dom: set<S>, codom: set<T>, rel: set<(S,T)>)
+
+            /*
+            Ensure that all values in tuples are from dom and codom
+            sets, respectively. 
+            */
+            requires forall x, y :: 
+                (x, y) in rel ==> x in dom && y in codom;
+
+            /*
+            Explain to verifier what this method accomplishes. The
+            verifier needs this information to verify propositions
+            elsewhere in this code. And because method bodies are 
+            "opaque" to the verifier, it can't read this information 
+            from the method body itself.
+            */
+            ensures d == dom && c == codom && r == rel;
+
+            /*
+            Once the constructor finishes, this object should 
+            satisfy its state invariant.
+            */
+            ensures Valid();
+        {
+            d := dom;
+            c := codom;
+            r := rel;
+        }
+
+        /*
+        Return domain/range set. 
+        */
+        function method dom(): set<S>
+            /*
+            The Dafny verifier needs to know what 
+            values function results depend on. So 
+            we have to tell it that the function
+            here can read any of the values (the
+            data members) in the current function.
+            */
+            reads this;
+            requires Valid();
+            ensures Valid();
+        {
+            d
+        }
+
+        /*
+        Return domain/range set
+        */
+        function method codom(): set<T>
+            reads this;
+            requires Valid();
+            ensures Valid();
+        {
+            c
+        }
+
+        /*
+        Return set of ordered pairs
+        */
+        function method rel(): set<(S,T)>
+            reads this
+            requires Valid();
+            ensures Valid();
+        {
+            r
+        }
+
+
+        /*
+        Return true iff the relation is single-valued (a function)
+        */
+        predicate method isFunction()
+            reads this;
+            requires Valid();
+            ensures Valid();
+        {
+            forall x, y, z :: x in d && y in c && z in c &&
+                            (x, y) in r && 
+                            (x, z) in r ==> 
+                            y == z  
+        }
+
+        
+        /*
+        Return true iff the relation is a function and is injective
+        */
+        predicate method isInjective()
+            reads this;
+            requires Valid();
+            requires isFunction();
+            ensures Valid();
+        {
+            forall x, y, z :: x in d && y in d && z in c &&
+                            (x, z) in r && 
+                            (y, z) in r ==> 
+                            x == y  
+        }
+        
+        
+        /*
+        Return true iff the relation is a function and is surjective 
+        */
+        predicate method isSurjective()
+            reads this;
+            requires Valid();
+            requires isFunction();
+            ensures Valid();
+        {
+            /*
+            Compute the set of all the y's in all the (x,y) pairs
+            in the relation, and see if that set is equal to t. If
+            so, then there is some tuple that "hits" every y in the
+            co-domain, and that's what it means to be surjective.
+            */
+            (set x, y | x in d && y in c && (x, y) in r :: y) == c    
+        }
+
+        /*
+        Return true iff the relation a function and is bijective
+        */
+
+        predicate method isBijective()
+            reads this;
+            requires Valid();
+            requires isFunction();
+            ensures Valid();
+        {
+            this.isInjective() && this.isSurjective()    
+        }
+
+
+       /*
+        Return true iff the relation is total (relative to its domain)
+        */
+        predicate method isTotal()
+            reads this;
+            requires Valid();
+            ensures Valid();
+        {
+            /*
+            Compare with isSurjective. Here we compute the set of all
+            the x's in all the (x,y) pairs, and if it's equal to the
+            domain, s, then this function is total (defined for every
+            value in s).
+            */
+            (set x, y | x in d && y in c && (x, y) in r :: x) == d
+        }
+
+        
+        /*
+        Return true iff the relation is partial (relative to its domain set)
+        */
+        predicate method isPartial()
+            reads this;
+            requires Valid();
+            ensures Valid();
+        {
+            !isTotal()
+        }
+
+
+        /*
+        */
+
+        predicate method inDomain(k: S)
+            requires Valid();
+            reads this;
+            ensures Valid();
+        {
+            k in dom()
+        }
+
+        predicate method inCodomain(v: T)
+            requires Valid();
+            reads this;
+            ensures Valid();
+        {
+            v in codom()
+        }
+
+        predicate method definedAt(k: S)
+            requires Valid()
+            requires k in d;
+            reads this;
+        {
+            // Check that cardinality of set of tuples with given key > 0
+            k in set x, y 
+                | x in dom() && y in codom() && (x, y) in rel() :: x
+        }
+
+
+        predicate method inRange(v: T)
+            requires Valid()
+            requires v in c;
+            reads this;
+        {
+            v in set x, y | 
+                x in dom() && y in codom() && (x, y) in rel() :: y 
+        }
+
+        /*
+        Compute image set of a value under this relation.
+        */
+        function method image(k: S): (vals: set<T>)
+            reads this;
+            requires Valid(); 
+            ensures Valid();
+        {
+            set x, y | x in d && y in c && (x, y) in r && x == k :: y
+        }
+
+
+        /*
+        Compute image of a domain element under this relation.
+        This code assumes there is exactly one element in the 
+        set from which the value is drawn, but this assumption
+        is not yet verified.
+        */
+        method imagef(k: S) returns (val: T)
+            requires Valid(); 
+            requires isFunction();  // ensures single-valuedness
+            requires k in d;        // ensures function is non-empty
+            requires definedAt(k);
+            ensures this == old(this);
+            ensures d == old(d) && c == old(c) && r == old(r);
+            ensures Valid();
+            /*
+            Make behavior of this opaque *method* visible as a spec
+            */
+            ensures val in set x, y | 
+                x in d && y in c && (x, y) in r && x == k :: y;
+        {
+            var s := set x, y | 
+                        x in d && y in c && (x, y) in r && x == k :: y;
+            val :| val in s;
+            // assert |s| == 1; -- believed true but doesn't verify
+        }
+    }
+}
